repatch/generated.c
@@ -55,6 +55,14 @@ extern unsigned int get_sub(unsigned int, unsigned int);
 
 extern unsigned int get_addr_ofs(unsigned long long, int);
 
+extern unsigned int get_block_ptr(struct memory_region *);
+
+extern unsigned int get_start_addr(struct memory_region *);
+
+extern unsigned int get_block_size(struct memory_region *);
+
+extern unsigned int get_block_perm(struct memory_region *);
+
 extern _Bool is_well_chunk_bool(unsigned int);
 
 extern unsigned int check_mem_aux2(struct memory_region *, unsigned int, unsigned int);
@@ -131,29 +139,29 @@ unsigned int reg64_to_reg32(unsigned long long d)
   return (unsigned int) d;
 }
 
-unsigned int get_src(unsigned long long ins$108)
+unsigned int get_src(unsigned long long ins$116)
 {
-  return (unsigned int) ((ins$108 & 65535LLU) >> 12LLU);
+  return (unsigned int) ((ins$116 & 65535LLU) >> 12LLU);
 }
 
-int get_offset(unsigned long long ins$110)
+int get_offset(unsigned long long ins$118)
 {
-  return (int) (short) (ins$110 << 32LLU >> 48LLU);
+  return (int) (short) (ins$118 << 32LLU >> 48LLU);
 }
 
-int get_immediate(unsigned long long ins$112)
+int get_immediate(unsigned long long ins$120)
 {
-  return (int) (ins$112 >> 32LLU);
+  return (int) (ins$120 >> 32LLU);
 }
 
-unsigned long long eval_immediate(int ins$114)
+unsigned long long eval_immediate(int ins$122)
 {
-  return (unsigned long long) ins$114;
+  return (unsigned long long) ins$122;
 }
 
-unsigned char get_opcode_ins(unsigned long long ins$116)
+unsigned char get_opcode_ins(unsigned long long ins$124)
 {
-  return (unsigned char) (ins$116 & 255LLU);
+  return (unsigned char) (ins$124 & 255LLU);
 }
 
 unsigned char get_opcode_alu64(unsigned char op)
@@ -161,39 +169,39 @@ unsigned char get_opcode_alu64(unsigned char op)
   return (unsigned char) (op & 240);
 }
 
-unsigned char get_opcode_alu32(unsigned char op$120)
+unsigned char get_opcode_alu32(unsigned char op$128)
 {
-  return (unsigned char) (op$120 & 240);
+  return (unsigned char) (op$128 & 240);
 }
 
-unsigned char get_opcode_branch(unsigned char op$122)
+unsigned char get_opcode_branch(unsigned char op$130)
 {
-  return (unsigned char) (op$122 & 240);
+  return (unsigned char) (op$130 & 240);
 }
 
-unsigned char get_opcode_mem_ld_imm(unsigned char op$124)
+unsigned char get_opcode_mem_ld_imm(unsigned char op$132)
 {
-  return (unsigned char) (op$124 & 255);
+  return (unsigned char) (op$132 & 255);
 }
 
-unsigned char get_opcode_mem_ld_reg(unsigned char op$126)
+unsigned char get_opcode_mem_ld_reg(unsigned char op$134)
 {
-  return (unsigned char) (op$126 & 255);
+  return (unsigned char) (op$134 & 255);
 }
 
-unsigned char get_opcode_mem_st_imm(unsigned char op$128)
+unsigned char get_opcode_mem_st_imm(unsigned char op$136)
 {
-  return (unsigned char) (op$128 & 255);
+  return (unsigned char) (op$136 & 255);
 }
 
-unsigned char get_opcode_mem_st_reg(unsigned char op$130)
+unsigned char get_opcode_mem_st_reg(unsigned char op$138)
 {
-  return (unsigned char) (op$130 & 255);
+  return (unsigned char) (op$138 & 255);
 }
 
-unsigned char get_opcode(unsigned char op$132)
+unsigned char get_opcode(unsigned char op$140)
 {
-  return (unsigned char) (op$132 & 7);
+  return (unsigned char) (op$140 & 7);
 }
 
 unsigned int get_add(unsigned int x, unsigned int y)
@@ -201,14 +209,34 @@ unsigned int get_add(unsigned int x, unsigned int y)
   return x + y;
 }
 
-unsigned int get_sub(unsigned int x$138, unsigned int y$140)
+unsigned int get_sub(unsigned int x$146, unsigned int y$148)
 {
-  return x$138 - y$140;
+  return x$146 - y$148;
 }
 
-unsigned int get_addr_ofs(unsigned long long x$142, int ofs)
+unsigned int get_addr_ofs(unsigned long long x$150, int ofs)
 {
-  return (unsigned int) (x$142 + (unsigned long long) (unsigned int) ofs);
+  return (unsigned int) (x$150 + (unsigned long long) (unsigned int) ofs);
+}
+
+unsigned int get_block_ptr(struct memory_region *mr)
+{
+  return (*mr).block_ptr;
+}
+
+unsigned int get_start_addr(struct memory_region *mr$156)
+{
+  return (*mr$156).start_addr;
+}
+
+unsigned int get_block_size(struct memory_region *mr$158)
+{
+  return (*mr$158).block_size;
+}
+
+unsigned int get_block_perm(struct memory_region *mr$160)
+{
+  return (*mr$160).block_perm;
 }
 
 _Bool is_well_chunk_bool(unsigned int chunk)
@@ -228,19 +256,24 @@ _Bool is_well_chunk_bool(unsigned int chunk)
   }
 }
 
-unsigned int check_mem_aux2(struct memory_region *mr, unsigned int addr, unsigned int chunk$152)
+unsigned int check_mem_aux2(struct memory_region *mr$164, unsigned int addr, unsigned int chunk$168)
 {
   _Bool well_chunk;
+  unsigned int ptr;
+  unsigned int start;
+  unsigned int size;
   unsigned int lo_ofs;
   unsigned int hi_ofs;
-  well_chunk = is_well_chunk_bool(chunk$152);
+  well_chunk = is_well_chunk_bool(chunk$168);
   if (well_chunk) {
-    lo_ofs = get_sub(addr, (*mr).start_addr);
-    hi_ofs = get_add(lo_ofs, (unsigned int) chunk$152);
-    if (0U <= lo_ofs && hi_ofs < (*mr).block_size) {
-      if (lo_ofs <= 4294967295U - (unsigned int) chunk$152
-            && 0U == lo_ofs % (unsigned int) chunk$152) {
-        return (*mr).block_ptr + lo_ofs;
+    ptr = get_block_ptr(mr$164);
+    start = get_start_addr(mr$164);
+    size = get_block_size(mr$164);
+    lo_ofs = get_sub(addr, start);
+    hi_ofs = get_add(lo_ofs, chunk$168);
+    if (0U <= lo_ofs && hi_ofs < size) {
+      if (lo_ofs <= 4294967295U - chunk$168 && 0U == lo_ofs % chunk$168) {
+        return ptr + lo_ofs;
       } else {
         return 0U;
       }
@@ -252,61 +285,63 @@ unsigned int check_mem_aux2(struct memory_region *mr, unsigned int addr, unsigne
   }
 }
 
-unsigned int check_mem_aux(unsigned int num, unsigned int perm, unsigned int chunk$164, unsigned int addr$166)
+unsigned int check_mem_aux(unsigned int num, unsigned int perm, unsigned int chunk$186, unsigned int addr$188)
 {
-  unsigned int n$168;
+  unsigned int n$190;
   struct memory_region *cur_mr;
-  unsigned int check_mem$172;
+  unsigned int mr_perm;
+  unsigned int check_mem$196;
   if (num == 0U) {
     return 0U;
   } else {
-    n$168 = num - 1U;
-    cur_mr = get_mem_region(n$168);
-    if ((*cur_mr).block_perm >= perm) {
-      check_mem$172 = check_mem_aux2(cur_mr, addr$166, chunk$164);
-      if (check_mem$172 == 0U) {
-        return check_mem_aux(n$168, perm, chunk$164, addr$166);
+    n$190 = num - 1U;
+    cur_mr = get_mem_region(n$190);
+    mr_perm = get_block_perm(cur_mr);
+    if (mr_perm >= perm) {
+      check_mem$196 = check_mem_aux2(cur_mr, addr$188, chunk$186);
+      if (check_mem$196 == 0U) {
+        return check_mem_aux(n$190, perm, chunk$186, addr$188);
       } else {
-        return check_mem$172;
+        return check_mem$196;
       }
     } else {
-      return check_mem_aux(n$168, perm, chunk$164, addr$166);
+      return check_mem_aux(n$190, perm, chunk$186, addr$188);
     }
   }
 }
 
-unsigned int check_mem(unsigned int perm$174, unsigned int chunk$176, unsigned int addr$178)
+unsigned int check_mem(unsigned int perm$198, unsigned int chunk$200, unsigned int addr$202)
 {
-  _Bool well_chunk$180;
+  _Bool well_chunk$204;
   unsigned int mem_reg_num;
-  unsigned int check_mem$184;
-  well_chunk$180 = is_well_chunk_bool(chunk$176);
-  if (well_chunk$180) {
+  unsigned int check_mem$208;
+  well_chunk$204 = is_well_chunk_bool(chunk$200);
+  if (well_chunk$204) {
     mem_reg_num = eval_mem_num();
-    check_mem$184 = check_mem_aux(mem_reg_num, perm$174, chunk$176, addr$178);
-    if (check_mem$184 == 0U) {
+    check_mem$208 = check_mem_aux(mem_reg_num, perm$198, chunk$200, addr$202);
+    if (check_mem$208 == 0U) {
       return 0U;
     } else {
-      return check_mem$184;
+      return check_mem$208;
     }
   } else {
     return 0U;
   }
 }
 
-_Bool comp_and_0x08_byte(unsigned char x$186)
+_Bool comp_and_0x08_byte(unsigned char x$210)
 {
-  return 0 == (x$186 & 8);
+  return 0 == (x$210 & 8);
 }
 
-void step_opcode_alu64(unsigned long long dst64, unsigned long long src64, unsigned int dst, unsigned char op$194)
+void step_opcode_alu64(unsigned long long dst64, unsigned long long src64, unsigned int dst, unsigned char op$218)
 {
   unsigned char opcode_alu64;
   unsigned int src32;
-  unsigned int src32$200;
-  unsigned int src32$202;
-  unsigned int src32$204;
-  opcode_alu64 = get_opcode_alu64(op$194);
+  unsigned int src32$224;
+  unsigned int src32$226;
+  unsigned int src32$228;
+  opcode_alu64 = get_opcode_alu64(op$218);
   switch (opcode_alu64) {
     case 0:
       upd_reg(dst, dst64 + src64);
@@ -348,9 +383,9 @@ void step_opcode_alu64(unsigned long long dst64, unsigned long long src64, unsig
         return;
       }
     case 112:
-      src32$200 = reg64_to_reg32(src64);
+      src32$224 = reg64_to_reg32(src64);
       if (src64 < 64LLU) {
-        upd_reg(dst, dst64 >> src32$200);
+        upd_reg(dst, dst64 >> src32$224);
         upd_flag(0);
         return;
       } else {
@@ -362,9 +397,9 @@ void step_opcode_alu64(unsigned long long dst64, unsigned long long src64, unsig
       upd_flag(0);
       return;
     case 144:
-      src32$202 = reg64_to_reg32(src64);
+      src32$226 = reg64_to_reg32(src64);
       if (src64 != 0LLU) {
-        upd_reg(dst, dst64 % src32$202);
+        upd_reg(dst, dst64 % src32$226);
         upd_flag(0);
         return;
       } else {
@@ -380,9 +415,9 @@ void step_opcode_alu64(unsigned long long dst64, unsigned long long src64, unsig
       upd_flag(0);
       return;
     case 192:
-      src32$204 = reg64_to_reg32(src64);
+      src32$228 = reg64_to_reg32(src64);
       if (src64 < 64LLU) {
-        upd_reg(dst, (long long) dst64 >> src32$204);
+        upd_reg(dst, (long long) dst64 >> src32$228);
         upd_flag(0);
         return;
       } else {
@@ -396,26 +431,26 @@ void step_opcode_alu64(unsigned long long dst64, unsigned long long src64, unsig
   }
 }
 
-void step_opcode_alu32(unsigned int dst32, unsigned int src32$208, unsigned int dst$210, unsigned char op$212)
+void step_opcode_alu32(unsigned int dst32, unsigned int src32$232, unsigned int dst$234, unsigned char op$236)
 {
   unsigned char opcode_alu32;
-  opcode_alu32 = get_opcode_alu32(op$212);
+  opcode_alu32 = get_opcode_alu32(op$236);
   switch (opcode_alu32) {
     case 0:
-      upd_reg(dst$210, (unsigned long long) (dst32 + src32$208));
+      upd_reg(dst$234, (unsigned long long) (dst32 + src32$232));
       upd_flag(0);
       return;
     case 16:
-      upd_reg(dst$210, (unsigned long long) (dst32 - src32$208));
+      upd_reg(dst$234, (unsigned long long) (dst32 - src32$232));
       upd_flag(0);
       return;
     case 32:
-      upd_reg(dst$210, (unsigned long long) (dst32 * src32$208));
+      upd_reg(dst$234, (unsigned long long) (dst32 * src32$232));
       upd_flag(0);
       return;
     case 48:
-      if (src32$208 != 0U) {
-        upd_reg(dst$210, (unsigned long long) (dst32 / src32$208));
+      if (src32$232 != 0U) {
+        upd_reg(dst$234, (unsigned long long) (dst32 / src32$232));
         upd_flag(0);
         return;
       } else {
@@ -423,16 +458,16 @@ void step_opcode_alu32(unsigned int dst32, unsigned int src32$208, unsigned int 
         return;
       }
     case 64:
-      upd_reg(dst$210, (unsigned long long) (dst32 | src32$208));
+      upd_reg(dst$234, (unsigned long long) (dst32 | src32$232));
       upd_flag(0);
       return;
     case 80:
-      upd_reg(dst$210, (unsigned long long) (dst32 & src32$208));
+      upd_reg(dst$234, (unsigned long long) (dst32 & src32$232));
       upd_flag(0);
       return;
     case 96:
-      if (src32$208 < 32U) {
-        upd_reg(dst$210, (unsigned long long) (dst32 << src32$208));
+      if (src32$232 < 32U) {
+        upd_reg(dst$234, (unsigned long long) (dst32 << src32$232));
         upd_flag(0);
         return;
       } else {
@@ -440,8 +475,8 @@ void step_opcode_alu32(unsigned int dst32, unsigned int src32$208, unsigned int 
         return;
       }
     case 112:
-      if (src32$208 < 32U) {
-        upd_reg(dst$210, (unsigned long long) (dst32 >> src32$208));
+      if (src32$232 < 32U) {
+        upd_reg(dst$234, (unsigned long long) (dst32 >> src32$232));
         upd_flag(0);
         return;
       } else {
@@ -449,12 +484,12 @@ void step_opcode_alu32(unsigned int dst32, unsigned int src32$208, unsigned int 
         return;
       }
     case 128:
-      upd_reg(dst$210, (unsigned long long) -dst32);
+      upd_reg(dst$234, (unsigned long long) -dst32);
       upd_flag(0);
       return;
     case 144:
-      if (src32$208 != 0U) {
-        upd_reg(dst$210, (unsigned long long) (dst32 % src32$208));
+      if (src32$232 != 0U) {
+        upd_reg(dst$234, (unsigned long long) (dst32 % src32$232));
         upd_flag(0);
         return;
       } else {
@@ -462,16 +497,16 @@ void step_opcode_alu32(unsigned int dst32, unsigned int src32$208, unsigned int 
         return;
       }
     case 160:
-      upd_reg(dst$210, (unsigned long long) (dst32 ^ src32$208));
+      upd_reg(dst$234, (unsigned long long) (dst32 ^ src32$232));
       upd_flag(0);
       return;
     case 176:
-      upd_reg(dst$210, src32$208);
+      upd_reg(dst$234, src32$232);
       upd_flag(0);
       return;
     case 192:
-      if (src32$208 < 32U) {
-        upd_reg(dst$210, (unsigned long long) ((int) dst32 >> src32$208));
+      if (src32$232 < 32U) {
+        upd_reg(dst$234, (unsigned long long) ((int) dst32 >> src32$232));
         upd_flag(0);
         return;
       } else {
@@ -485,18 +520,18 @@ void step_opcode_alu32(unsigned int dst32, unsigned int src32$208, unsigned int 
   }
 }
 
-void step_opcode_branch(unsigned long long dst64$216, unsigned long long src64$218, int pc, int ofs$222, unsigned char op$224)
+void step_opcode_branch(unsigned long long dst64$240, unsigned long long src64$242, int pc, int ofs$246, unsigned char op$248)
 {
   unsigned char opcode_jmp;
-  opcode_jmp = get_opcode_branch(op$224);
+  opcode_jmp = get_opcode_branch(op$248);
   switch (opcode_jmp) {
     case 0:
-      upd_pc(pc + ofs$222);
+      upd_pc(pc + ofs$246);
       upd_flag(0);
       return;
     case 16:
-      if (dst64$216 == src64$218) {
-        upd_pc(pc + ofs$222);
+      if (dst64$240 == src64$242) {
+        upd_pc(pc + ofs$246);
         upd_flag(0);
         return;
       } else {
@@ -504,8 +539,8 @@ void step_opcode_branch(unsigned long long dst64$216, unsigned long long src64$2
         return;
       }
     case 32:
-      if (dst64$216 > src64$218) {
-        upd_pc(pc + ofs$222);
+      if (dst64$240 > src64$242) {
+        upd_pc(pc + ofs$246);
         upd_flag(0);
         return;
       } else {
@@ -513,8 +548,8 @@ void step_opcode_branch(unsigned long long dst64$216, unsigned long long src64$2
         return;
       }
     case 48:
-      if (dst64$216 >= src64$218) {
-        upd_pc(pc + ofs$222);
+      if (dst64$240 >= src64$242) {
+        upd_pc(pc + ofs$246);
         upd_flag(0);
         return;
       } else {
@@ -522,8 +557,8 @@ void step_opcode_branch(unsigned long long dst64$216, unsigned long long src64$2
         return;
       }
     case 160:
-      if (dst64$216 < src64$218) {
-        upd_pc(pc + ofs$222);
+      if (dst64$240 < src64$242) {
+        upd_pc(pc + ofs$246);
         upd_flag(0);
         return;
       } else {
@@ -531,8 +566,8 @@ void step_opcode_branch(unsigned long long dst64$216, unsigned long long src64$2
         return;
       }
     case 176:
-      if (dst64$216 <= src64$218) {
-        upd_pc(pc + ofs$222);
+      if (dst64$240 <= src64$242) {
+        upd_pc(pc + ofs$246);
         upd_flag(0);
         return;
       } else {
@@ -540,8 +575,8 @@ void step_opcode_branch(unsigned long long dst64$216, unsigned long long src64$2
         return;
       }
     case 64:
-      if ((dst64$216 & src64$218) != 0LLU) {
-        upd_pc(pc + ofs$222);
+      if ((dst64$240 & src64$242) != 0LLU) {
+        upd_pc(pc + ofs$246);
         upd_flag(0);
         return;
       } else {
@@ -549,8 +584,8 @@ void step_opcode_branch(unsigned long long dst64$216, unsigned long long src64$2
         return;
       }
     case 80:
-      if (dst64$216 != src64$218) {
-        upd_pc(pc + ofs$222);
+      if (dst64$240 != src64$242) {
+        upd_pc(pc + ofs$246);
         upd_flag(0);
         return;
       } else {
@@ -558,8 +593,8 @@ void step_opcode_branch(unsigned long long dst64$216, unsigned long long src64$2
         return;
       }
     case 96:
-      if ((long long) dst64$216 > (long long) src64$218) {
-        upd_pc(pc + ofs$222);
+      if ((long long) dst64$240 > (long long) src64$242) {
+        upd_pc(pc + ofs$246);
         upd_flag(0);
         return;
       } else {
@@ -567,8 +602,8 @@ void step_opcode_branch(unsigned long long dst64$216, unsigned long long src64$2
         return;
       }
     case 112:
-      if ((long long) dst64$216 >= (long long) src64$218) {
-        upd_pc(pc + ofs$222);
+      if ((long long) dst64$240 >= (long long) src64$242) {
+        upd_pc(pc + ofs$246);
         upd_flag(0);
         return;
       } else {
@@ -576,8 +611,8 @@ void step_opcode_branch(unsigned long long dst64$216, unsigned long long src64$2
         return;
       }
     case 192:
-      if ((long long) dst64$216 < (long long) src64$218) {
-        upd_pc(pc + ofs$222);
+      if ((long long) dst64$240 < (long long) src64$242) {
+        upd_pc(pc + ofs$246);
         upd_flag(0);
         return;
       } else {
@@ -585,8 +620,8 @@ void step_opcode_branch(unsigned long long dst64$216, unsigned long long src64$2
         return;
       }
     case 208:
-      if ((long long) dst64$216 <= (long long) src64$218) {
-        upd_pc(pc + ofs$222);
+      if ((long long) dst64$240 <= (long long) src64$242) {
+        upd_pc(pc + ofs$246);
         upd_flag(0);
         return;
       } else {
@@ -603,18 +638,18 @@ void step_opcode_branch(unsigned long long dst64$216, unsigned long long src64$2
   }
 }
 
-void step_opcode_mem_ld_imm(int imm, int pc$230, int len, unsigned int dst$234, unsigned char op$236, unsigned long long *l$238)
+void step_opcode_mem_ld_imm(int imm, int pc$254, int len, unsigned int dst$258, unsigned char op$260, unsigned long long *l$262)
 {
   unsigned char opcode_ld;
   unsigned long long next_ins;
   int next_imm;
-  opcode_ld = get_opcode_mem_ld_imm(op$236);
+  opcode_ld = get_opcode_mem_ld_imm(op$260);
   switch (opcode_ld) {
     case 24:
-      if (pc$230 + 1 < len) {
-        next_ins = list_get(l$238, pc$230 + 1);
+      if (pc$254 + 1 < len) {
+        next_ins = list_get(l$262, pc$254 + 1);
         next_imm = get_immediate(next_ins);
-        upd_reg(dst$234,
+        upd_reg(dst$258,
                 (unsigned long long) (unsigned int) imm
                   | (unsigned long long) (unsigned int) next_imm << 32U);
         upd_pc_incr();
@@ -631,116 +666,60 @@ void step_opcode_mem_ld_imm(int imm, int pc$230, int len, unsigned int dst$234, 
   }
 }
 
-void step_opcode_mem_ld_reg(unsigned int addr$246, int pc$248, unsigned int dst$250, unsigned char op$252)
+void step_opcode_mem_ld_reg(unsigned int addr$270, int pc$272, unsigned int dst$274, unsigned char op$276)
 {
-  unsigned char opcode_ld$254;
+  unsigned char opcode_ld$278;
   unsigned int addr_ptr;
   unsigned long long v;
-  unsigned int addr_ptr$260;
-  unsigned long long v$262;
-  unsigned int addr_ptr$264;
-  unsigned long long v$266;
-  unsigned int addr_ptr$268;
-  unsigned long long v$270;
-  opcode_ld$254 = get_opcode_mem_ld_reg(op$252);
-  switch (opcode_ld$254) {
+  unsigned int addr_ptr$284;
+  unsigned long long v$286;
+  unsigned int addr_ptr$288;
+  unsigned long long v$290;
+  unsigned int addr_ptr$292;
+  unsigned long long v$294;
+  opcode_ld$278 = get_opcode_mem_ld_reg(op$276);
+  switch (opcode_ld$278) {
     case 97:
-      addr_ptr = check_mem(1U, 4U, addr$246);
+      addr_ptr = check_mem(1U, 4U, addr$270);
       if (addr_ptr == 0U) {
         upd_flag(-2);
         return;
       } else {
         v = load_mem(4U, addr_ptr);
-        upd_reg(dst$250, v);
+        upd_reg(dst$274, v);
         upd_flag(0);
         return;
       }
     case 105:
-      addr_ptr$260 = check_mem(1U, 2U, addr$246);
-      if (addr_ptr$260 == 0U) {
-        upd_flag(-2);
-        return;
-      } else {
-        v$262 = load_mem(2U, addr_ptr$260);
-        upd_reg(dst$250, v$262);
-        upd_flag(0);
-        return;
-      }
-    case 113:
-      addr_ptr$264 = check_mem(1U, 1U, addr$246);
-      if (addr_ptr$264 == 0U) {
-        upd_flag(-2);
-        return;
-      } else {
-        v$266 = load_mem(1U, addr_ptr$264);
-        upd_reg(dst$250, v$266);
-        upd_flag(0);
-        return;
-      }
-    case 121:
-      addr_ptr$268 = check_mem(1U, 8U, addr$246);
-      if (addr_ptr$268 == 0U) {
-        upd_flag(-2);
-        return;
-      } else {
-        v$270 = load_mem(8U, addr_ptr$268);
-        upd_reg(dst$250, v$270);
-        upd_flag(0);
-        return;
-      }
-    default:
-      upd_flag(-1);
-      return;
-    
-  }
-}
-
-void step_opcode_mem_st_imm(int imm$272, unsigned int addr$274, int pc$276, unsigned int dst$278, unsigned char op$280)
-{
-  unsigned char opcode_st;
-  unsigned int addr_ptr$284;
-  unsigned int addr_ptr$286;
-  unsigned int addr_ptr$288;
-  unsigned int addr_ptr$290;
-  opcode_st = get_opcode_mem_st_imm(op$280);
-  switch (opcode_st) {
-    case 98:
-      addr_ptr$284 = check_mem(2U, 4U, addr$274);
+      addr_ptr$284 = check_mem(1U, 2U, addr$270);
       if (addr_ptr$284 == 0U) {
         upd_flag(-2);
         return;
       } else {
-        store_mem_imm(4U, addr_ptr$284, imm$272);
+        v$286 = load_mem(2U, addr_ptr$284);
+        upd_reg(dst$274, v$286);
         upd_flag(0);
         return;
       }
-    case 106:
-      addr_ptr$286 = check_mem(2U, 2U, addr$274);
-      if (addr_ptr$286 == 0U) {
-        upd_flag(-2);
-        return;
-      } else {
-        store_mem_imm(2U, addr_ptr$286, imm$272);
-        upd_flag(0);
-        return;
-      }
-    case 114:
-      addr_ptr$288 = check_mem(2U, 1U, addr$274);
+    case 113:
+      addr_ptr$288 = check_mem(1U, 1U, addr$270);
       if (addr_ptr$288 == 0U) {
         upd_flag(-2);
         return;
       } else {
-        store_mem_imm(1U, addr_ptr$288, imm$272);
+        v$290 = load_mem(1U, addr_ptr$288);
+        upd_reg(dst$274, v$290);
         upd_flag(0);
         return;
       }
-    case 122:
-      addr_ptr$290 = check_mem(2U, 8U, addr$274);
-      if (addr_ptr$290 == 0U) {
+    case 121:
+      addr_ptr$292 = check_mem(1U, 8U, addr$270);
+      if (addr_ptr$292 == 0U) {
         upd_flag(-2);
         return;
       } else {
-        store_mem_imm(8U, addr_ptr$290, imm$272);
+        v$294 = load_mem(8U, addr_ptr$292);
+        upd_reg(dst$274, v$294);
         upd_flag(0);
         return;
       }
@@ -751,52 +730,52 @@ void step_opcode_mem_st_imm(int imm$272, unsigned int addr$274, int pc$276, unsi
   }
 }
 
-void step_opcode_mem_st_reg(unsigned long long src64$292, unsigned int addr$294, int pc$296, unsigned int dst$298, unsigned char op$300)
+void step_opcode_mem_st_imm(int imm$296, unsigned int addr$298, int pc$300, unsigned int dst$302, unsigned char op$304)
 {
-  unsigned char opcode_st$302;
-  unsigned int addr_ptr$304;
-  unsigned int addr_ptr$306;
+  unsigned char opcode_st;
   unsigned int addr_ptr$308;
   unsigned int addr_ptr$310;
-  opcode_st$302 = get_opcode_mem_st_reg(op$300);
-  switch (opcode_st$302) {
-    case 99:
-      addr_ptr$304 = check_mem(2U, 4U, addr$294);
-      if (addr_ptr$304 == 0U) {
-        upd_flag(-2);
-        return;
-      } else {
-        store_mem_reg(4U, addr_ptr$304, src64$292);
-        upd_flag(0);
-        return;
-      }
-    case 107:
-      addr_ptr$306 = check_mem(2U, 2U, addr$294);
-      if (addr_ptr$306 == 0U) {
-        upd_flag(-2);
-        return;
-      } else {
-        store_mem_reg(2U, addr_ptr$306, src64$292);
-        upd_flag(0);
-        return;
-      }
-    case 115:
-      addr_ptr$308 = check_mem(2U, 1U, addr$294);
+  unsigned int addr_ptr$312;
+  unsigned int addr_ptr$314;
+  opcode_st = get_opcode_mem_st_imm(op$304);
+  switch (opcode_st) {
+    case 98:
+      addr_ptr$308 = check_mem(2U, 4U, addr$298);
       if (addr_ptr$308 == 0U) {
         upd_flag(-2);
         return;
       } else {
-        store_mem_reg(1U, addr_ptr$308, src64$292);
+        store_mem_imm(4U, addr_ptr$308, imm$296);
         upd_flag(0);
         return;
       }
-    case 123:
-      addr_ptr$310 = check_mem(2U, 8U, addr$294);
+    case 106:
+      addr_ptr$310 = check_mem(2U, 2U, addr$298);
       if (addr_ptr$310 == 0U) {
         upd_flag(-2);
         return;
       } else {
-        store_mem_reg(8U, addr_ptr$310, src64$292);
+        store_mem_imm(2U, addr_ptr$310, imm$296);
+        upd_flag(0);
+        return;
+      }
+    case 114:
+      addr_ptr$312 = check_mem(2U, 1U, addr$298);
+      if (addr_ptr$312 == 0U) {
+        upd_flag(-2);
+        return;
+      } else {
+        store_mem_imm(1U, addr_ptr$312, imm$296);
+        upd_flag(0);
+        return;
+      }
+    case 122:
+      addr_ptr$314 = check_mem(2U, 8U, addr$298);
+      if (addr_ptr$314 == 0U) {
+        upd_flag(-2);
+        return;
+      } else {
+        store_mem_imm(8U, addr_ptr$314, imm$296);
         upd_flag(0);
         return;
       }
@@ -807,135 +786,191 @@ void step_opcode_mem_st_reg(unsigned long long src64$292, unsigned int addr$294,
   }
 }
 
-void step(int len$312, unsigned long long *l$314)
+void step_opcode_mem_st_reg(unsigned long long src64$316, unsigned int addr$318, int pc$320, unsigned int dst$322, unsigned char op$324)
 {
-  int pc$316;
-  unsigned long long ins$318;
-  unsigned char op$320;
-  unsigned char opc;
-  unsigned int dst$324;
-  unsigned long long dst64$326;
-  _Bool is_imm;
-  int imm$330;
-  unsigned long long imm64;
-  unsigned int src;
-  unsigned long long src64$336;
-  unsigned int dst$338;
-  unsigned long long dst64$340;
-  unsigned int dst32$342;
-  _Bool is_imm$344;
-  int imm$346;
-  unsigned int src$348;
-  unsigned long long src64$350;
-  unsigned int src32$352;
-  unsigned int dst$354;
-  unsigned long long dst64$356;
-  int ofs$358;
-  _Bool is_imm$360;
-  int imm$362;
-  unsigned long long imm64$364;
-  unsigned int src$366;
-  unsigned long long src64$368;
-  unsigned int dst$370;
-  int imm$372;
-  unsigned int dst$374;
-  unsigned int src$376;
-  unsigned long long src64$378;
-  int ofs$380;
-  unsigned int addr$382;
-  unsigned int dst$384;
-  unsigned long long dst64$386;
-  int ofs$388;
-  int imm$390;
-  unsigned int addr$392;
-  unsigned int dst$394;
-  unsigned long long dst64$396;
-  unsigned int src$398;
-  unsigned long long src64$400;
-  int ofs$402;
-  unsigned int addr$404;
-  pc$316 = eval_pc();
-  ins$318 = list_get(l$314, pc$316);
-  op$320 = get_opcode_ins(ins$318);
-  opc = get_opcode(op$320);
-  switch (opc) {
-    case 7:
-      dst$324 = get_dst(ins$318);
-      dst64$326 = eval_reg(dst$324);
-      is_imm = comp_and_0x08_byte(op$320);
-      if (is_imm) {
-        imm$330 = get_immediate(ins$318);
-        imm64 = eval_immediate(imm$330);
-        step_opcode_alu64(dst64$326, imm64, dst$324, op$320);
+  unsigned char opcode_st$326;
+  unsigned int addr_ptr$328;
+  unsigned int addr_ptr$330;
+  unsigned int addr_ptr$332;
+  unsigned int addr_ptr$334;
+  opcode_st$326 = get_opcode_mem_st_reg(op$324);
+  switch (opcode_st$326) {
+    case 99:
+      addr_ptr$328 = check_mem(2U, 4U, addr$318);
+      if (addr_ptr$328 == 0U) {
+        upd_flag(-2);
         return;
       } else {
-        src = get_src(ins$318);
-        src64$336 = eval_reg(src);
-        step_opcode_alu64(dst64$326, src64$336, dst$324, op$320);
+        store_mem_reg(4U, addr_ptr$328, src64$316);
+        upd_flag(0);
+        return;
+      }
+    case 107:
+      addr_ptr$330 = check_mem(2U, 2U, addr$318);
+      if (addr_ptr$330 == 0U) {
+        upd_flag(-2);
+        return;
+      } else {
+        store_mem_reg(2U, addr_ptr$330, src64$316);
+        upd_flag(0);
+        return;
+      }
+    case 115:
+      addr_ptr$332 = check_mem(2U, 1U, addr$318);
+      if (addr_ptr$332 == 0U) {
+        upd_flag(-2);
+        return;
+      } else {
+        store_mem_reg(1U, addr_ptr$332, src64$316);
+        upd_flag(0);
+        return;
+      }
+    case 123:
+      addr_ptr$334 = check_mem(2U, 8U, addr$318);
+      if (addr_ptr$334 == 0U) {
+        upd_flag(-2);
+        return;
+      } else {
+        store_mem_reg(8U, addr_ptr$334, src64$316);
+        upd_flag(0);
+        return;
+      }
+    default:
+      upd_flag(-1);
+      return;
+    
+  }
+}
+
+void step(int len$336, unsigned long long *l$338)
+{
+  int pc$340;
+  unsigned long long ins$342;
+  unsigned char op$344;
+  unsigned char opc;
+  unsigned int dst$348;
+  unsigned long long dst64$350;
+  _Bool is_imm;
+  int imm$354;
+  unsigned long long imm64;
+  unsigned int src;
+  unsigned long long src64$360;
+  unsigned int dst$362;
+  unsigned long long dst64$364;
+  unsigned int dst32$366;
+  _Bool is_imm$368;
+  int imm$370;
+  unsigned int src$372;
+  unsigned long long src64$374;
+  unsigned int src32$376;
+  unsigned int dst$378;
+  unsigned long long dst64$380;
+  int ofs$382;
+  _Bool is_imm$384;
+  int imm$386;
+  unsigned long long imm64$388;
+  unsigned int src$390;
+  unsigned long long src64$392;
+  unsigned int dst$394;
+  int imm$396;
+  unsigned int dst$398;
+  unsigned int src$400;
+  unsigned long long src64$402;
+  int ofs$404;
+  unsigned int addr$406;
+  unsigned int dst$408;
+  unsigned long long dst64$410;
+  int ofs$412;
+  int imm$414;
+  unsigned int addr$416;
+  unsigned int dst$418;
+  unsigned long long dst64$420;
+  unsigned int src$422;
+  unsigned long long src64$424;
+  int ofs$426;
+  unsigned int addr$428;
+  pc$340 = eval_pc();
+  ins$342 = list_get(l$338, pc$340);
+  op$344 = get_opcode_ins(ins$342);
+  opc = get_opcode(op$344);
+  switch (opc) {
+    case 7:
+      dst$348 = get_dst(ins$342);
+      dst64$350 = eval_reg(dst$348);
+      is_imm = comp_and_0x08_byte(op$344);
+      if (is_imm) {
+        imm$354 = get_immediate(ins$342);
+        imm64 = eval_immediate(imm$354);
+        step_opcode_alu64(dst64$350, imm64, dst$348, op$344);
+        return;
+      } else {
+        src = get_src(ins$342);
+        src64$360 = eval_reg(src);
+        step_opcode_alu64(dst64$350, src64$360, dst$348, op$344);
         return;
       }
     case 4:
-      dst$338 = get_dst(ins$318);
-      dst64$340 = eval_reg(dst$338);
-      dst32$342 = reg64_to_reg32(dst64$340);
-      is_imm$344 = comp_and_0x08_byte(op$320);
-      if (is_imm$344) {
-        imm$346 = get_immediate(ins$318);
-        step_opcode_alu32(dst32$342, imm$346, dst$338, op$320);
+      dst$362 = get_dst(ins$342);
+      dst64$364 = eval_reg(dst$362);
+      dst32$366 = reg64_to_reg32(dst64$364);
+      is_imm$368 = comp_and_0x08_byte(op$344);
+      if (is_imm$368) {
+        imm$370 = get_immediate(ins$342);
+        step_opcode_alu32(dst32$366, imm$370, dst$362, op$344);
         return;
       } else {
-        src$348 = get_src(ins$318);
-        src64$350 = eval_reg(src$348);
-        src32$352 = reg64_to_reg32(src64$350);
-        step_opcode_alu32(dst32$342, src32$352, dst$338, op$320);
+        src$372 = get_src(ins$342);
+        src64$374 = eval_reg(src$372);
+        src32$376 = reg64_to_reg32(src64$374);
+        step_opcode_alu32(dst32$366, src32$376, dst$362, op$344);
         return;
       }
     case 5:
-      dst$354 = get_dst(ins$318);
-      dst64$356 = eval_reg(dst$354);
-      ofs$358 = get_offset(ins$318);
-      is_imm$360 = comp_and_0x08_byte(op$320);
-      if (is_imm$360) {
-        imm$362 = get_immediate(ins$318);
-        imm64$364 = eval_immediate(imm$362);
-        step_opcode_branch(dst64$356, imm64$364, pc$316, ofs$358, op$320);
+      dst$378 = get_dst(ins$342);
+      dst64$380 = eval_reg(dst$378);
+      ofs$382 = get_offset(ins$342);
+      is_imm$384 = comp_and_0x08_byte(op$344);
+      if (is_imm$384) {
+        imm$386 = get_immediate(ins$342);
+        imm64$388 = eval_immediate(imm$386);
+        step_opcode_branch(dst64$380, imm64$388, pc$340, ofs$382, op$344);
         return;
       } else {
-        src$366 = get_src(ins$318);
-        src64$368 = eval_reg(src$366);
-        step_opcode_branch(dst64$356, src64$368, pc$316, ofs$358, op$320);
+        src$390 = get_src(ins$342);
+        src64$392 = eval_reg(src$390);
+        step_opcode_branch(dst64$380, src64$392, pc$340, ofs$382, op$344);
         return;
       }
     case 0:
-      dst$370 = get_dst(ins$318);
-      imm$372 = get_immediate(ins$318);
-      step_opcode_mem_ld_imm(imm$372, pc$316, len$312, dst$370, op$320,
-                             l$314);
+      dst$394 = get_dst(ins$342);
+      imm$396 = get_immediate(ins$342);
+      step_opcode_mem_ld_imm(imm$396, pc$340, len$336, dst$394, op$344,
+                             l$338);
       return;
     case 1:
-      dst$374 = get_dst(ins$318);
-      src$376 = get_src(ins$318);
-      src64$378 = eval_reg(src$376);
-      ofs$380 = get_offset(ins$318);
-      addr$382 = get_addr_ofs(src64$378, ofs$380);
-      step_opcode_mem_ld_reg(addr$382, pc$316, dst$374, op$320);
+      dst$398 = get_dst(ins$342);
+      src$400 = get_src(ins$342);
+      src64$402 = eval_reg(src$400);
+      ofs$404 = get_offset(ins$342);
+      addr$406 = get_addr_ofs(src64$402, ofs$404);
+      step_opcode_mem_ld_reg(addr$406, pc$340, dst$398, op$344);
       return;
     case 2:
-      dst$384 = get_dst(ins$318);
-      dst64$386 = eval_reg(dst$384);
-      ofs$388 = get_offset(ins$318);
-      imm$390 = get_immediate(ins$318);
-      addr$392 = get_addr_ofs(dst64$386, ofs$388);
-      step_opcode_mem_st_imm(imm$390, addr$392, pc$316, dst$384, op$320);
+      dst$408 = get_dst(ins$342);
+      dst64$410 = eval_reg(dst$408);
+      ofs$412 = get_offset(ins$342);
+      imm$414 = get_immediate(ins$342);
+      addr$416 = get_addr_ofs(dst64$410, ofs$412);
+      step_opcode_mem_st_imm(imm$414, addr$416, pc$340, dst$408, op$344);
       return;
     case 3:
-      dst$394 = get_dst(ins$318);
-      dst64$396 = eval_reg(dst$394);
-      src$398 = get_src(ins$318);
-      src64$400 = eval_reg(src$398);
-      ofs$402 = get_offset(ins$318);
-      addr$404 = get_addr_ofs(dst64$396, ofs$402);
-      step_opcode_mem_st_reg(src64$400, addr$404, pc$316, dst$394, op$320);
+      dst$418 = get_dst(ins$342);
+      dst64$420 = eval_reg(dst$418);
+      src$422 = get_src(ins$342);
+      src64$424 = eval_reg(src$422);
+      ofs$426 = get_offset(ins$342);
+      addr$428 = get_addr_ofs(dst64$420, ofs$426);
+      step_opcode_mem_st_reg(src64$424, addr$428, pc$340, dst$418, op$344);
       return;
     default:
       upd_flag(-1);
@@ -944,23 +979,23 @@ void step(int len$312, unsigned long long *l$314)
   }
 }
 
-void bpf_interpreter_aux(int len$406, unsigned int fuel, unsigned long long *l$410)
+void bpf_interpreter_aux(int len$430, unsigned int fuel, unsigned long long *l$434)
 {
   unsigned int fuel0;
-  int pc$414;
+  int pc$438;
   int f;
   if (fuel == 0U) {
     upd_flag(-5);
     return;
   } else {
     fuel0 = fuel - 1U;
-    pc$414 = eval_pc();
-    if (0U <= pc$414 && pc$414 < len$406) {
-      step(len$406, l$410);
+    pc$438 = eval_pc();
+    if (0U <= pc$438 && pc$438 < len$430) {
+      step(len$430, l$434);
       upd_pc_incr();
       f = eval_flag();
       if (f == 0) {
-        bpf_interpreter_aux(len$406, fuel0, l$410);
+        bpf_interpreter_aux(len$430, fuel0, l$434);
         return;
       } else {
         return;
@@ -972,15 +1007,15 @@ void bpf_interpreter_aux(int len$406, unsigned int fuel, unsigned long long *l$4
   }
 }
 
-unsigned long long bpf_interpreter(int len$418, unsigned int fuel$420, unsigned long long *l$422)
+unsigned long long bpf_interpreter(int len$442, unsigned int fuel$444, unsigned long long *l$446)
 {
   struct memory_region *bpf_ctx;
-  int f$426;
+  int f$450;
   bpf_ctx = get_mem_region(0U);
   upd_reg(1U, (*bpf_ctx).start_addr);
-  bpf_interpreter_aux(len$418, fuel$420, l$422);
-  f$426 = eval_flag();
-  if (f$426 == 1) {
+  bpf_interpreter_aux(len$442, fuel$444, l$446);
+  f$450 = eval_flag();
+  if (f$450 == 1) {
     return eval_reg(0U);
   } else {
     return 0LLU;
