proof/correctproof/correct_get_add_chunk.v
@@ -1,33 +1,29 @@
 From bpf.src Require Import DxIntegers DxValues DxMemRegion DxState DxMonad DxInstructions.
-From Coq Require Import List Lia.
+From Coq Require Import List Lia ZArith.
 From compcert Require Import Integers Values Clight Memory.
 Import ListNotations.
-Require Import ZArith.
 
 From bpf.proof Require Import Clightlogic MatchState CorrectRel CommonLemma.
 
-From bpf.benchmark Require Import clightlogicexample.
+From bpf.clight Require Import interpreter.
 
 (**
-unsigned int get_add(unsigned int x, unsigned int y)
-{
-  return x + y;
-}
+Print get_add.
 
 get_add = 
 fun x y : valu32_t => returnM (Val.add x y)
-     : valu32_t -> valu32_t -> M valu32_t
+     : valu32_t -> val -> M valu32_t
 
 *)
 
-Section Get_add.
+Section Get_add_chunk.
 
   (** The program contains our function of interest [fn] *)
   Definition p : Clight.program := prog.
 
   (* [Args,Res] provides the mapping between the Coq and the C types *)
   (* Definition Args : list CompilableType := [stateCompilableType].*)
-  Definition args : list Type := [(valu32_t:Type); (valu32_t:Type)].
+  Definition args : list Type := [(valu32_t:Type); (val:Type)].
   Definition res : Type := (valu32_t:Type).
 
   (* [f] is a Coq Monadic function with the right type *)
@@ -47,7 +43,7 @@ Section Get_add.
   (* [match_res] relates the Coq result and the C result *)
   Definition match_res : res -> val -> stateM -> Memory.Mem.mem -> Prop := fun x v st m => valu32_correct x v.
 
-  Instance correct_function3_get_add : forall a, correct_function3 p args res f fn (nil) true match_arg_list match_res a.
+  Instance correct_function3_get_add_chunk : forall a, correct_function3 p args res f fn (nil) true match_arg_list match_res a.
   Proof.
     intros. unfold args in a.
     car_cdr.
@@ -61,19 +57,15 @@ Section Get_add.
     get_invariant_more _y.
 
     unfold stateless, valu32_correct in H1, H3.
-    destruct H1 as (Hc_eq & (vi & Hvi_eq)).
-    destruct H3 as (Hc0_eq & (vj & Hvj_eq)).
-    subst c c0 v v0.
+    completer.
+    subst.
 
-    (**according to the c function:
-unsigned int get_add(unsigned int x, unsigned int y)
-{
-  return x + y;
-}
+    (**according to the type of eval_pc:
+         static unsigned long long get_addl(unsigned long long x, unsigned long long y)
        1. return value should be  x+y
        2. the memory is same
       *)
-    exists (Val.add (Vint vi) (Vint vj)), m, Events.E0.
+    exists (Val.add (Vint x0) (Vint x)), m, Events.E0.
 
     repeat split; unfold step2.
     -
@@ -85,6 +77,6 @@ unsigned int get_add(unsigned int x, unsigned int y)
       reflexivity.
   Qed.
 
-End Get_add.
+End Get_add_chunk.
 
-Existing Instance correct_function3_get_add.
+Existing Instance correct_function3_get_add_chunk.
