proof/correctproof/correct_is_well_chunk_bool.v
@@ -8,7 +8,7 @@ Import ListNotations.
 
 From bpf.proof Require Import clight_exec Clightlogic CorrectRel MatchState CommonLemma.
 
-From bpf.benchmark Require Import clightlogicexample.
+From bpf.clight Require Import interpreter.
 
 
 Definition match_state (st_block : block) (_ : unit) (v : val) (st: stateM) (m : Memory.Mem.mem) : Prop :=
@@ -22,8 +22,8 @@ Variable st_block : block.
 Definition p : Clight.program := prog.
 
 (* [Args,Res] provides the mapping between the Coq and the C types *)
-Definition Args : list Type := [memory_chunk:Type].
-Definition Res : Type := bool.
+Definition args : list Type := [memory_chunk:Type].
+Definition res : Type := bool.
 
 (* [f] is a Coq Monadic function with the right type *)
 Definition f := is_well_chunk_bool.
@@ -40,9 +40,11 @@ Ltac exec_seq_of_labeled_statement :=
       change (seq_of_labeled_statement X) with x
   end.
 
-Instance correct_function_is_well_chunk_bool2 : correct_function3
-    p Args Res f fn [] true (DList.DCons  (stateless match_chunk) (DList.DNil _)) (stateless match_bool).
+Instance correct_function_is_well_chunk_bool2 : forall a, correct_function3
+    p args res f fn [] true (DList.DCons  (stateless match_chunk) (DList.DNil _)) (stateless match_bool) a.
 Proof.
+  intros. unfold args in a.
+  car_cdr.
   correct_function_from_body.
   correct_body.
   unfold INV, f.
@@ -57,9 +59,11 @@ Proof.
 
   exists (Vint (if v' then Integers.Int.one else Integers.Int.zero)).
   exists m, Events.E0.
+  
   repeat split; unfold step2.
   -
-    unfold Int.one in *.
+    unfold memory_chunk_to_valu32, well_chunk_Z in p0, H2.
+    unfold align_chunk in p0, H2.
     destruct c; inv Heq; simpl.
     all: try
     forward_star;
@@ -72,6 +76,57 @@ Proof.
     destruct v' ; reflexivity.
 Qed.
 
+(*
+Instance correct_function_is_well_chunk_bool2 : forall unmod,
+  correct_function3
+    p Args Res f fn unmod true (DList.DCons  (stateless match_chunk) (DList.DNil _)) (stateless match_bool).
+Proof.
+  intro.
+  correct_function_from_body.
+  repeat intro.
+  simpl in H.
+  unfold Args in a.
+  car_cdr.
+  unfold list_rel_arg in H.
+  simpl in H.
+  unfold app.
+  unfold f,f_is_well_chunk_bool.
+  destruct (is_well_chunk_bool c st) eqn:E ; auto.
+  destruct p0 as (v',st'); intros.
+  unfold fn at 2. unfold f_is_well_chunk_bool.
+  unfold fn_body.
+  get_invariant _chunk.
+  destruct c0 as [MC  C].
+  unfold stateless in MC.
+  unfold match_chunk in MC.
+  subst.
+  exists (Vint (if v' then Integers.Int.one else Integers.Int.zero)).
+  exists m. exists Events.E0.
+  repeat split.
+  + eapply Smallstep.star_step; eauto.
+    econstructor; eauto.
+    econstructor;eauto.
+    constructor.
+    unfold Integers.Int.one.
+    destruct c;inv E.
+    Ltac switch :=
+      match goal with
+        |- context[Integers.Int.unsigned (Integers.Int.repr ?X)] =>
+          change (Integers.Int.unsigned (Integers.Int.repr X)) with X;
+          exec_seq_of_labeled_statement
+      end;
+      eapply Smallstep.star_step; eauto;
+      [econstructor;eauto |
+        eapply Smallstep.star_step; eauto ; [econstructor; eauto;
+                                            econstructor; eauto|]
+      ]; apply Smallstep.star_refl.
+    all: try switch.
+    reflexivity.
+  + simpl.
+    constructor.
+    destruct v' ; reflexivity.
+Qed.
+*)
 End Is_well_chunk_bool.
 
 Existing Instance correct_function_is_well_chunk_bool2.
